src/Assembly/Pseudize.v
@@ -8,27 +8,38 @@ Import Pseudo ListNotations StateCommon EvalUtil ListState.
 Section Conversion.
 
   Hint Unfold setList getList getVar setCarry setCarryOpt getCarry
-       getMem setMem overflows.
+       getMem setMem overflows ensureLength.
 
   Lemma eval_in_length: forall {w s n m} p x M c x' M' c',
       @pseudoEval n m w s p (x, M, c) = Some (x', M', c')
     -> Datatypes.length x = n.
-  Proof. Admitted.
-
-  Lemma eval_out_length: forall {w s n m} x M c x' M' c' p,
-      @pseudoEval n m w s p (x, M, c) = Some (x', M', c')
-    -> Datatypes.length x' = m.
-  Proof. Admitted.
-
-  Lemma pseudo_var: forall {w s n} b k x v m c,
-      (k < n)%nat
-    -> nth_error x k = Some v
-    -> pseudoEval (@PVar w s n b (indexize k)) (x, m, c) = Some ([v], m, c).
   Proof.
-    intros; autounfold; simpl; unfold indexize.
+    autounfold; intros until c'; intro H.
+    destruct (Nat.eq_dec (Datatypes.length (getList (x, M, c))) n)
+      as [Hn|Hn].
+
+    - intuition.
+    - assert (pseudoEval p (x, M, c) = None) as H0.
+      induction p; simpl; unfold ensureLength;
+        destruct (Nat.eq_dec _ n);
+        simpl; intuition.
+      rewrite H in H0; inversion H0.
+  Qed.
+
+  Lemma pseudo_var: forall {w s n} b k x v m m' c c',
+      (k < n)%nat -> m = m' -> c = c' -> Datatypes.length x = n
+    -> nth_error x k = Some v
+    -> pseudoEval (@PVar w s n b (indexize k)) (x, m, c) =
+        Some ([v], m', c').
+  Proof.
+    intros until c'.
+    intros B r0 r1 H H0; rewrite r0, r1.
+
+    autounfold; simpl; unfold indexize.
     destruct (le_dec n 0); simpl. {
       replace k with 0 in * by omega; autounfold; simpl in *.
       rewrite H0; simpl; intuition.
+      destruct (Nat.eq_dec _ n); try rewrite H0; intuition.
     }
 
     replace (k mod n) with k by (
@@ -39,25 +50,35 @@ Section Conversion.
 
     autounfold; simpl.
     destruct (nth_error x k); simpl; try inversion H0; intuition.
+    destruct (Nat.eq_dec _ n); intuition.
   Qed.
 
   Lemma pseudo_mem: forall {w s} n v m c x name len index,
-      TripleM.find (w, name mod n, index mod len)%nat m = Some (@wordToN w v)
+      Datatypes.length x = n
+    -> TripleM.find (w, name mod n, index mod len)%nat m = Some (@wordToN w v)
     -> pseudoEval (@PMem w s n len (indexize name) (indexize index)) (x, m, c) = Some ([v], m, c).
   Proof.
-    intros; autounfold; simpl.
+    intros until index; intros H H0; autounfold; simpl.
     unfold indexize;
       destruct (le_dec n 0), (le_dec len 0);
       try replace n with 0 in * by intuition;
       try replace len with 0 in * by intuition;
-      autounfold; simpl in *; rewrite H;
+      autounfold; simpl in *; rewrite H0;
       autounfold; simpl; rewrite NToWord_wordToN;
-      intuition.
+      intuition; rewrite H;
+      destruct (Nat.eq_dec _ n); simpl in *;
+      try omega; intuition.
   Qed.
 
   Lemma pseudo_const: forall {w s n} x v m c,
-      pseudoEval (@PConst w s n v) (x, m, c) = Some ([v], m, c).
-  Proof. intros; simpl; intuition. Qed.
+      Datatypes.length x = n
+    -> pseudoEval (@PConst w s n v) (x, m, c) = Some ([v], m, c).
+  Proof.
+    intros;
+      unfold pseudoEval, ensureLength; autounfold;
+      simpl; rewrite H; intuition.
+    destruct (Nat.eq_dec _ n); simpl; intuition.
+  Qed.
 
   Lemma pseudo_plus:
     forall {w s n} (p: @Pseudo w s n 2) x out0 out1 m0 m1 c0 c1,
@@ -67,12 +88,16 @@ Section Conversion.
           Some (proj1_sig (bool_of_sumbool
                (overflows w (&out0 + &out1)%N)%w))).
   Proof.
-    intros; simpl; rewrite H; simpl.
+    intros until c1; intro H; simpl; rewrite H; simpl.
 
     pose proof (wordize_plus out0 out1).
     destruct (overflows w _); autounfold; simpl; try rewrite H0;
       try rewrite <- (@Npow2_ignore w (out0 ^+ out1));
-      try rewrite NToWord_wordToN; intuition.
+      try rewrite NToWord_wordToN; intuition;
+
+      apply eval_in_length in H;
+      destruct (Nat.eq_dec (Datatypes.length x) n);
+      intuition; inversion H.
   Qed.
 
   Lemma pseudo_bin:
@@ -82,12 +107,15 @@ Section Conversion.
     -> pseudoEval (PBin n op p) (x, m0, c0) =
         Some ([fst (evalIntOp op out0 out1)], m1, c1).
   Proof.
-    intros; simpl; rewrite H0; simpl.
+    intros until op; intros H H0; simpl; rewrite H0; simpl.
 
-    induction op;
+    autounfold; induction op;
       try (contradict H; reflexivity);
       unfold evalIntOp; autounfold; simpl;
-      reflexivity.
+
+      apply eval_in_length in H0;
+      destruct (Nat.eq_dec (Datatypes.length x) n);
+      intuition.
   Qed.
 
   Lemma pseudo_and:
@@ -113,9 +141,12 @@ Section Conversion.
     intros; simpl; rewrite H; simpl.
 
     pose proof (wordize_awc out0 out1); unfold evalCarryOp.
-    destruct (overflows w ((& out0)%w + (& out1)%w +
-                           (if c then 1%N else 0%N)));
-      autounfold; simpl; try rewrite H0; intuition.
+    destruct (overflows w _);
+      autounfold; simpl; try rewrite H0; intuition;
+
+      apply eval_in_length in H;
+      destruct (Nat.eq_dec _ n);
+      intuition.
   Qed.
 
   Lemma pseudo_shiftr:
@@ -126,6 +157,10 @@ Section Conversion.
   Proof.
     intros; simpl; rewrite H; autounfold; simpl.
     rewrite wordize_shiftr; rewrite NToWord_wordToN; intuition.
+
+    apply eval_in_length in H;
+      destruct (Nat.eq_dec _ n);
+      intuition.
   Qed.
 
   Lemma pseudo_comb:
@@ -139,13 +174,17 @@ Section Conversion.
     intros; autounfold; simpl.
     rewrite H; autounfold; simpl.
     rewrite H0; autounfold; simpl; intuition.
+
+    apply eval_in_length in H;
+      destruct (Nat.eq_dec _ n);
+      intuition.
   Qed.
 
   Lemma pseudo_cons:
     forall {w s n b} (p0: @Pseudo w s n 1) (p1: @Pseudo w s n b)
         (p2: @Pseudo w s n (S b)) input x xs m0 m1 m2 c0 c1 c2,
-      pseudoEval p0 (input, m0, c0) = Some ([x], m1, c1)
-    -> pseudoEval p1 (input, m1, c1) = Some (xs, m2, c2)
+      pseudoEval p1 (input, m1, c1) = Some (xs, m2, c2)
+    -> pseudoEval p0 (input, m0, c0) = Some ([x], m1, c1)
     -> p2 = (@PComb w s n _ _ p0 p1)
     -> pseudoEval p2 (input, m0, c0) = Some (x :: xs, m2, c2).
   Proof.
@@ -166,6 +205,10 @@ Section Conversion.
     intros; autounfold; simpl.
     rewrite H; autounfold; simpl.
     rewrite H0; autounfold; simpl; intuition.
+
+    apply eval_in_length in H;
+      destruct (Nat.eq_dec _ n);
+      intuition.
   Qed.
 
   Lemma pseudo_let_var:
@@ -209,11 +252,14 @@ Section Conversion.
     -> pseudoEval (@PLet w s n 2 m (PDual n Mult p0) p1) (x, m0, c0) =
       Some (Let_In (out0 ^* out1) f, m2, c2).
   Proof.
-    intros; simpl; rewrite H; autounfold; simpl; rewrite H0; simpl; intuition.
+    intros until c2; intros H H0; simpl; rewrite H; autounfold; simpl.
+
+    apply eval_in_length in H;
+      destruct (Nat.eq_dec _ n);
+      simpl; try rewrite H0; simpl; intuition.
+
     replace (nth n (x ++ _) _) with (out0 ^* out1); simpl; intuition.
-    assert (Datatypes.length x = n) as L by (
-      eapply eval_in_length; eassumption).
-    rewrite app_nth2; try rewrite L; intuition.
+    rewrite app_nth2; try rewrite H; intuition.
     replace (n - n) with 0 by omega.
     simpl; intuition.
   Qed.
@@ -232,17 +278,20 @@ Section Conversion.
             Let_In (out0 ^* out1) (fun y =>
             f y x)), m2, c2).
   Proof.
-    intros; simpl; rewrite H; autounfold; simpl; rewrite H0; simpl; intuition.
-    assert (Datatypes.length x = n) as L by (eapply eval_in_length; eassumption).
+    intros until c2; intros H H0; simpl; rewrite H; autounfold; simpl.
+
+    apply eval_in_length in H;
+      destruct (Nat.eq_dec _ n);
+      simpl; try rewrite H0; simpl; intuition.
 
     replace (nth n (x ++ _) _) with (out0 ^* out1); simpl; intuition.
     replace (nth (S n) (x ++ _) _) with (multHigh out0 out1); simpl; intuition.
 
-    - rewrite app_nth2; try rewrite L; intuition.
+    - rewrite app_nth2; try rewrite H; intuition.
       replace (S n - n) with 1 by omega.
       simpl; intuition.
 
-    - rewrite app_nth2; try rewrite L; intuition.
+    - rewrite app_nth2; try rewrite H; intuition.
       replace (n - n) with 0 by omega.
       simpl; intuition.
   Qed.
@@ -299,11 +348,14 @@ Ltac pseudo_step :=
 
   | [ |- @pseudoEval ?n _ _ _ ?P _ =
         Some ([nth ?i ?lst _], _, _)%p ] =>
-    eapply (pseudo_var None i); simpl; intuition
+    eapply (pseudo_var None i);
+      try reflexivity; autodestruct;
+      simpl; intuition
   end.
 
 Ltac pseudo_solve :=
   repeat eexists;
   autounfold;
   autodestruct;
-  repeat pseudo_step.
+  repeat pseudo_step;
+  intuition.
